Modularise Eval

Semantic/Fsub/Eval.lean
@@ -1,64 +1,8 @@
-import Semantic.Fsub.Syntax
-import Semantic.Fsub.Substitution
-
-namespace Fsub
+import Semantic.Fsub.Eval.Core
+import Semantic.Fsub.Eval.BasicProps
 
 /-!
-A store is a list of locally-closed expressions.
+# Fsub Evaluation
+
+This module re-exports the core evaluation definitions and basic properties.
 -/
-inductive Store : Type where
-| nil : Store
-| cons : Val {} -> Store -> Store
-
-def Store.lookup : Store -> Nat -> Option (Val {})
-| .cons v _, 0 => some v
-| .cons _ s, n+1 => Store.lookup s n
-| .nil, _ => none
-
-def Store.snoc : Store -> Val {} -> Store
-| .cons v s, v0 => .cons v (s.snoc v0)
-| .nil, v => .cons v nil
-
-def Store.append : Store -> Store -> Store
-| .nil, s2 => s2
-| .cons v s1, s2 => .cons v (s1.append s2)
-
-instance Store.instAppend : Append Store where
-  append := Store.append
-
-def Store.len : Store -> Nat
-| .cons _ s => s.len + 1
-| .nil => 0
-
-inductive Step : Store -> Exp {} -> Store -> Exp {} -> Prop where
-| st_ctx :
-  Step s1 e1 s2 e2 ->
-  Step s1 (.letin e1 u) s2 (.letin e2 u)
-| st_apply :
-  s1.lookup x = some ⟨.abs T e, hv⟩ ->
-  Step s1 (.app (.free x) y) s1 (e.subst (Subst.openVar y))
-| st_tapply :
-  s1.lookup x = some ⟨.tabs T0 e, hv⟩ ->
-  Step s1 (.tapp (.free x) T) s1 (e.subst (Subst.openTVar .top))
-| st_rename :
-  Step s1 (.letin (.var x) e) s1 (e.subst (Subst.openVar x))
-| st_lift :
-  (hv : Exp.IsVal v) ->
-  Step s1 (.letin v e) (s1.snoc ⟨v, hv⟩) (e.subst (Subst.openVar (.free s1.len)))
-
-inductive Reduce : Store -> Exp {} -> Store -> Exp {} -> Prop where
-| red_refl :
-  Reduce s e s e
-| red_step :
-  Step s e s' e' ->
-  Reduce s' e' s'' e'' ->
-  Reduce s e s'' e''
-
-inductive Exp.IsAns : Exp {} -> Prop where
-| is_val :
-  (hv : Exp.IsVal v) ->
-  Exp.IsAns v
-| is_var :
-  Exp.IsAns (.var x)
-
-end Fsub
